continue hnr automation

Array_Safe.thy
@@ -1,6 +1,8 @@
 theory Array_Safe
-  imports Base
+  imports  Diff_Arr
 begin
+
+(* TODO: Use locale? *)
 
 definition array_nth_safe where
   "array_nth_safe arr i = do {
@@ -21,6 +23,26 @@ definition array_update_safe where
     else return arr
   }"
 
+definition diff_arr_lookup_safe where
+  "diff_arr_lookup_safe arr i = do {
+    len \<leftarrow>  Diff_Arr.length arr;
+    if i < len
+    then  Diff_Arr.lookup arr i
+    else do { 
+      arr \<leftarrow>  Diff_Arr.realize arr;
+      xs \<leftarrow> Array.freeze arr;
+      return (xs ! i)
+    }
+  }"
+
+definition diff_arr_update_safe  where
+  "diff_arr_update_safe arr i v = do {
+    len \<leftarrow>  Diff_Arr.length arr;
+    if i < len
+    then Diff_Arr.update arr i v 
+    else return arr
+  }"
+
 lemma nth_undefined: "i \<ge> length xs \<Longrightarrow> xs ! i = undefined(i - length xs)"
   apply(induction xs arbitrary: i)
   unfolding List.nth_def
@@ -38,5 +60,34 @@ lemma array_update_safe [sep_heap_rules]:
   unfolding array_update_safe_def
   by sep_auto
 
+lemma update_safe[sep_heap_rules]: "
+  <master_assn t * \<up>(t \<turnstile> xs \<sim> diff_arr)> 
+     diff_arr_update_safe diff_arr i v
+  <\<lambda>diff_arr. \<exists>\<^sub>At'. master_assn t' * 
+    \<up>((\<forall>xs' diff_arr'. t \<turnstile> xs' \<sim> diff_arr' \<longrightarrow> t' \<turnstile> xs' \<sim> diff_arr') 
+      \<and> (t' \<turnstile> xs[i := v] \<sim> diff_arr))>\<^sub>t
+"
+  unfolding diff_arr_update_safe_def
+  apply sep_auto
+   apply(rule fi_rule[OF length])
+   apply sep_auto
+  apply sep_auto
+   apply(rule cons_post_rule)
+    apply(rule fi_rule[OF update])
+  by sep_auto+
+
+lemma lookup_safe [sep_heap_rules]: "
+  <master_assn t * \<up>(t \<turnstile> xs \<sim> a)> 
+     diff_arr_lookup_safe a i 
+  <\<lambda>r. master_assn t * \<up>(r = xs!i)>\<^sub>t"
+  unfolding diff_arr_lookup_safe_def
+  apply sep_auto
+   apply(rule fi_rule[OF length])
+   apply sep_auto+
+  apply(rule cons_post_rule)
+    apply(rule fi_rule[OF lookup])
+    apply sep_auto+
+   apply(rule fi_rule[OF realize])
+  by sep_auto+
 
 end
