Test.thy
@@ -1,5 +1,5 @@
 theory Test
-  imports Diff_Arr HNR "HOL-Library.Code_Target_Nat"
+  imports Diff_Arr HNR "HOL-Library.Code_Target_Nat" 
 begin
 
 (* Diff Array *)
@@ -7,14 +7,14 @@ begin
 definition create_diff_arr where
   "create_diff_arr n x = do {
     a \<leftarrow> Array.new n x;
-    from_array a
+    Diff_Arr.from_array a
   }"
 
 definition test where "test = do {
   r \<leftarrow> create_diff_arr 3 (5::nat);
-  y  \<leftarrow> update r 1 (7::nat);
-  y' \<leftarrow> update r 1 (8::nat);
-  x \<leftarrow> lookup y 1;
+  y  \<leftarrow> Diff_Arr.update r 1 (7::nat);
+  y' \<leftarrow> Diff_Arr.update r 1 (8::nat);
+  x \<leftarrow> Diff_Arr.lookup y 1;
   return x
 }"
 
@@ -30,67 +30,220 @@ definition test1 where
   "test1 xs = 
     (let c1 = (let x = 1 in x); c2 = 2; c3 = 3; t1 = xs[c1 := c2]; t2 = t1[c1 := c3]; t3 = t2 ! c2 in t3)"
 
+definition test2 where
+  "test2 xs = 
+    (let c1 = 1; t1 = xs[c1 := c1] in t1)"
+
 attribute_setup framed =
     \<open>Scan.succeed (Thm.rule_attribute [] (fn _ => fn thm => @{thm hnr_frame} OF [asm_rl, thm]))\<close>
     \<open>Add frame to hnr rule\<close>
 
 thm hnr_rule[framed]
 
-method hnr_rule = 
-  (rule hnr_rule[framed] hnr_copy[framed] hnr_return[framed], (frame_inference; fail))
+lemma frame_inference_trivial: "P \<Longrightarrow>\<^sub>A P * emp"
+  by sep_auto
 
-method hnr_rule_2 = 
-  (rule hnr_rule_2[framed] hnr_copy[framed], (frame_inference; fail)) | (rule hnr_let hnr_return)
+method frame_inference' = rule frame_inference_trivial | frame_inference
+
+
+ 
+
+
+lemma move_pure_right: 
+  "a * (b * c) = (a * b) * c" 
+  "NO_MATCH (\<up>(x)) b \<Longrightarrow> \<up>(p) * b = b * \<up>(p)"
+  "NO_MATCH (\<up>(x)) b \<Longrightarrow> a * \<up>(p) * b = a * b * \<up>(p)"
+  by(auto simp: algebra_simps)  
+
+lemma hnr_pre_cong: "\<Gamma> = \<Gamma>' \<Longrightarrow> hnr \<Gamma> c \<Gamma>'' R a = hnr \<Gamma>' c \<Gamma>'' R a"
+  by simp
+
+lemma hnr_extract_pure:
+  assumes
+    "p \<Longrightarrow> hnr \<Gamma> c \<Gamma>' R a"
+  shows 
+    "hnr (\<Gamma> * \<up>(p)) c \<Gamma>' R a"
+  using assms 
+  unfolding hnr_def
+  apply(cases p) 
+  by auto
+
+(* hnr_pre_cong ent_refl *)
+
+
+lemma prepare_frame_1:
+  assumes
+    "emp * P * emp \<Longrightarrow>\<^sub>A emp * Q * F"
+  shows
+    "P \<Longrightarrow>\<^sub>A Q * F"
+  using assms
+  by sep_auto
+
+lemma frame_no_match: 
+  assumes
+    "Ps1 * (P * Ps2) \<Longrightarrow>\<^sub>A Qs * Q * F"
+  shows
+    "Ps1 * P * Ps2 \<Longrightarrow>\<^sub>A Qs * Q * F"
+  using assms
+  by (simp add: mult.assoc)
+
+lemma frame_match_pure:
+  assumes
+    "Ps1 * \<up>(P) * Ps2 \<Longrightarrow>\<^sub>A Qs * F"
+  shows
+    "Ps1 * \<up>(P) * Ps2 \<Longrightarrow>\<^sub>A Qs * \<up>(P) * F"
+  using assms
+  by simp
+
+lemma frame_match:
+  assumes
+    "Ps1 * Ps2 \<Longrightarrow>\<^sub>A Qs * F"
+  shows
+    "Ps1 * P * Ps2 \<Longrightarrow>\<^sub>A Qs * P * F"
+  using assms
+  by (metis assn_aci(10) fr_refl)
+
+lemma frame_match_emp:
+   assumes
+    "Ps \<Longrightarrow>\<^sub>A Qs * F"
+  shows
+    "Ps \<Longrightarrow>\<^sub>A Qs * emp * F"
+  using assms
+  by sep_auto
+
+lemma frame_done: "F * emp \<Longrightarrow>\<^sub>A emp * F" 
+  by sep_auto
+
+find_theorems "_ * emp"
+
+method frame_norm_assoc = (simp only: mult.left_assoc[where 'a=assn])?
+
+method frame_prepare = rule prepare_frame_1, frame_norm_assoc
+
+method frame_try_match = then_else \<open>rule frame_match_pure frame_match frame_match_emp\<close> \<open>frame_norm_assoc\<close> \<open>rule frame_no_match, frame_try_match\<close>
+
+method frame_done = simp only: assn_one_left mult_1_right[where 'a=assn], rule ent_refl  
+
+method frame_inference_2 = frame_prepare, frame_try_match+, frame_done
+
+method frame_inference_2_dbg = frame_prepare, (frame_try_match+)?, frame_done?
+
+method hnr_rule = 
+  (rule hnr_rule[framed] hnr_copy[framed] hnr_return[framed], (frame_inference'; fail))
+
+thm  hnr_return[of emp, framed]
 
 method hnr_rule_diff_arr =
-  (rule hnr_rule_diff_arr[framed] hnr_copy[framed], (frame_inference; fail)) | (rule hnr_let hnr_return)
+  (rule hnr_rule_diff_arr[framed] hnr_copy[framed], frame_inference_2) | rule hnr_return
 
 method hnr = (hnr_rule | keep_drop)+
-
-method hnr_2 = (hnr_rule_2 | keep_drop)+
 
 method hnr_diff_arr = (hnr_rule_diff_arr | keep_drop)+
 
 schematic_goal "hnr (array_assn xs xsi) (?c :: ?'a Heap) ?\<Gamma>' ?R (test1 xs)"
-  by hnr_2
+   unfolding test1_def
+   by hnr
+
+(* lemma norm_pre_ex_rule:
+  assumes A: "\<And>x. <P x> f <Q>"
+  shows "<\<exists>\<^sub>Ax. P x> f <Q>" 
+*)
+
+lemma hnr_exE: 
+  assumes "\<And>x. hnr (\<Gamma> x) c \<Gamma>' R a"
+  shows "hnr (\<exists>\<^sub>Ax. \<Gamma> x) c \<Gamma>' R a"
+  using assms norm_pre_ex_rule
+  unfolding hnr_def
+  by sep_auto
+
+experiment
+begin
+
+schematic_goal 
+  fixes a b c d::assn
+  shows "a * b * c * d \<Longrightarrow>\<^sub>A a * c * ?F"
+    apply frame_inference_2
+  done
+
+schematic_goal 
+  fixes a b c d::assn
+  shows "a * b * c * d \<Longrightarrow>\<^sub>A emp * ?F"
+   apply frame_inference_2
+  done
+
+schematic_goal 
+  fixes a b c d::assn
+  shows "emp \<Longrightarrow>\<^sub>A emp * ?F"
+   apply frame_inference_2
+  done
+
+schematic_goal 
+  fixes a b c d::assn
+  shows "a * b * c * d \<Longrightarrow>\<^sub>A b * d * ?F"
+   apply frame_inference_2
+  done
+
+schematic_goal 
+ 
+  shows "a * \<up>(b) * c * d \<Longrightarrow>\<^sub>A \<up>(b) * d * ?F"
+   apply frame_inference_2
+  done
+
+end
+
+method normalize_hnr_pre = simp(no_asm) named_ss HOL_basic_ss_nomatch:
+  move_pure_right assn_one_left mult_1_right[where 'a=assn] cong: hnr_pre_cong
+
+(*method frame_inference_init_2 = ((rule hnr_extract_pure move_pure_right)+)? 
+method frame_inference_match_2 = ((rule hnr_pre_cong ent_refl)+)?
+
+method frame_inference_2 = frame_inference_init_2, frame_inference_match_2
+
+method hnr_rule_diff_arr_2 =
+  (rule hnr_rule_diff_arr[framed] hnr_copy[framed] hnr_return[framed], (frame_inference_2))*)
 
 schematic_goal "hnr (array_assn xs xsi) (?c :: ?'a Heap) ?\<Gamma>' ?R (test1 xs)"
   unfolding test1_def 
-  apply(rule hnr_let)
-  apply(rule hnr_let)
-  apply(rule hnr_return)
-  apply(rule hnr_copy[framed], frame_inference)
-  apply keep_drop
-     (* Here: *)
-   (* apply(rule hnr_let[framed])
-  apply(frame_inference) *)
-  apply(rule hnr_let)
-  apply(rule hnr_return)
-  apply(rule hnr_let)
-  apply(rule hnr_return)
-  apply(rule hnr_let)
-  apply(rule hnr_array_update[framed], frame_inference)
-  apply(rule hnr_let)
-  apply(rule hnr_array_update[framed], frame_inference)
-  apply(rule hnr_let)
-  apply(rule hnr_array_nth[framed], frame_inference)
-  apply(rule hnr_copy[framed], frame_inference)
-  by keep_drop+
-
-schematic_goal "hnr (array_assn xs xsi) (?c :: ?'a Heap) ?\<Gamma>' ?R (test1 xs)"
-  unfolding test1_def 
+  by hnr
+ 
+schematic_goal "hnr (master_assn t * \<up>(t \<turnstile> xs \<sim> xsi)) (?c :: ?'a Heap) ?\<Gamma>' ?R (test1 xs)"
+  unfolding test1_def
+  apply (hnr_rule_diff_arr)
+  apply (hnr_rule_diff_arr)
+      apply (hnr_rule_diff_arr)  
+     apply (hnr_rule_diff_arr)
+    apply keep_drop
   apply(hnr_rule_diff_arr)
+     apply(hnr_rule_diff_arr)
+    (* TODO: Keep pure left, because non-linear use *)
     apply(hnr_rule_diff_arr)
       apply(hnr_rule_diff_arr)
      apply(hnr_rule_diff_arr)
-  apply keep_drop
-   apply(hnr_rule_diff_arr)
      apply(hnr_rule_diff_arr)
-    apply(hnr_rule_diff_arr)
-      apply(hnr_rule_diff_arr)
-     apply(hnr_rule_diff_arr)
-  (* How to get to master_assn in the first place? *)
-       apply(rule hnr_update'[framed])
+  back
+     apply frame_prepare
+  apply frame_try_match
+     apply(hnr_rule_diff_arr, frame_inference_2)
+ apply(hnr_rule_diff_arr, frame_inference_2)
+ apply(hnr_rule_diff_arr, frame_inference_2)
+  apply(hnr_rule_diff_arr, frame_inference_2)
+ apply(hnr_rule_diff_arr, frame_inference_2_dbg)
+       apply(rule hnr_rule_diff_arr[framed])
+  apply normalize_hnr_pre
+        apply frame_inference_2
+   find_theorems "<\<exists>\<^sub>A _. _> _ <_>"
+       apply(simp only: ex_assn_move_out, intro hnr_exE)
+
+       apply hnr_rule_diff_arr
+         apply(rule hnr_rule_diff_arr[framed])
+    apply FI_keep
+   sorry
+
+schematic_goal "hnr (array_assn xs xsi) (?c :: ?'a Heap) ?\<Gamma>' ?R (test2 xs)"
+  unfolding test2_def 
+  apply hnr
+     apply(rule hnr_rule[framed])
+  apply frame_inference
   sorry
 
 export_code array_nth_safe array_update_safe in SML_imp
