More_Eisbach_Tools.thy
@@ -1,0 +1,235 @@
+theory More_Eisbach_Tools
+imports "HOL-Eisbach.Eisbach" Automatic_Refinement.Refine_Util
+begin
+
+section \<open>More Tracing\<close>
+
+(* Copied from Eisbach_Tools *)
+ML \<open>
+
+val cfg_trace_level = Attrib.setup_config_int @{binding vcg_trace_level} (K 0)
+
+local
+
+fun trace_method parser print =
+  Scan.lift (Parse.int) -- parser >>
+    (fn (lvl,x) => fn ctxt => SIMPLE_METHOD (fn st =>
+      (if not (Method.detect_closure_state st) andalso Config.get ctxt cfg_trace_level >= lvl
+       then tracing (print ctxt x st) else ();
+       all_tac st)));
+
+    
+val trace_goal_method = trace_method 
+  (Scan.lift (Scan.optional Parse.text ""))
+  (fn ctxt => fn msg => fn st => 
+    let
+      val t = Logic.get_goal (Thm.prop_of st) 1
+    in
+      Pretty.block [
+        Pretty.str msg, Pretty.str ":", Pretty.brk 1, 
+        Pretty.str (Syntax.string_of_term ctxt t)
+      ]
+      |> Pretty.string_of
+    end
+  )
+    
+val trace_msg_method = trace_method (Scan.lift Parse.text) (K (fn msg => K msg))
+    
+in
+
+val _ =
+  Theory.setup
+   (  Method.setup @{binding vcg_trace_goal} trace_goal_method ""
+   #> Method.setup @{binding vcg_trace_msg} trace_msg_method ""
+   );
+
+end
+\<close>
+
+(*
+section \<open>Method Result Determinization\<close>
+text \<open>The \<open>DETERM\<close> combinator on method level\<close>
+method_setup determ = \<open>
+  Method.text_closure >>
+    (fn (text) => fn ctxt => fn using => fn st =>
+      Seq.DETERM (Method.evaluate_runtime text ctxt using) st
+    )
+\<close>
+*)
+
+(*
+section \<open>Combinators in Upcoming Isabelle (2018) Release\<close>
+
+ML \<open>fun method_evaluate text ctxt facts =
+  Method.NO_CONTEXT_TACTIC ctxt
+    (Method.evaluate_runtime text ctxt facts)\<close>
+
+method_setup all =
+ \<open>Method.text_closure >> (fn m => fn ctxt => fn facts =>
+   let
+     fun tac i st' =
+       Goal.restrict i 1 st'
+       |> method_evaluate m ctxt facts
+       |> Seq.map (Goal.unrestrict i)
+
+   in SIMPLE_METHOD (ALLGOALS tac) facts end)
+\<close>
+
+method_setup determ =
+ \<open>Method.text_closure >> (fn m => fn ctxt => fn facts =>
+   let
+     fun tac st' = method_evaluate m ctxt facts st'
+
+   in SIMPLE_METHOD (DETERM tac) facts end)
+\<close>
+
+method_setup changed =
+ \<open>Method.text_closure >> (fn m => fn ctxt => fn facts =>
+   let
+     fun tac st' = method_evaluate m ctxt facts st'
+
+   in SIMPLE_METHOD (CHANGED tac) facts end)
+\<close>
+*)
+
+
+subsection \<open>Deterministic Repeated Elimination Rule\<close>
+text \<open>Attention: Slightly different semantics than @{method elim}: repeats the 
+  rule as long as possible, but only on the first subgoal.\<close>
+method_setup vcg_elim_determ = \<open>
+  Attrib.thms >> (fn thms => fn ctxt => 
+    SIMPLE_METHOD (REPEAT_DETERM1 (HEADGOAL (ematch_tac ctxt thms))))\<close>
+
+    
+subsection \<open>If-Then-Else\<close>    
+(*
+  TODO: Improve handling of seq. Currently, the first result is determinised
+
+*)
+method_setup then_else = \<open>let
+in
+  Method.text_closure -- Method.text_closure -- Method.text_closure >>
+    (fn ((textb, textt), texte) => fn ctxt => fn using => fn st =>
+      let
+        val bmethod = Method.evaluate_runtime textb ctxt using;
+        val tmethod = Method.evaluate_runtime textt ctxt using;
+        val emethod = Method.evaluate_runtime texte ctxt using;
+      in
+        (case try (fn st => bmethod st |> Seq.pull) st of
+          SOME (SOME (Seq.Result st,_)) => tmethod st
+        | _ => emethod st)
+      end)
+end     
+\<close>
+    
+method_setup solved_then_else = \<open>let
+  infix 0 SOLVED_THEN_ELSE
+
+  fun (tac1 SOLVED_THEN_ELSE (tac2,tac3)) st =
+    tac1 st 
+    |> Seq.maps (fn st' => 
+         if Thm.nprems_of st' < Thm.nprems_of st then tac2 st' (* Solved goal *)
+         else tac3 st' (* Did not solve goal *)
+       )
+
+in
+  Method.text_closure -- Method.text_closure -- Method.text_closure >>
+    (fn ((textb, textt), texte) => fn ctxt => fn using =>
+      let
+        val bmethod = method_evaluate textb ctxt [];
+        val tmethod = method_evaluate textt ctxt [];
+        val emethod = method_evaluate texte ctxt [];
+      in
+        SIMPLE_METHOD (bmethod SOLVED_THEN_ELSE (tmethod, emethod)) using
+      end)
+end     
+\<close>
+
+
+
+method_setup then_all_new_fwd =
+ \<open>Method.text_closure -- Method.text_closure >> (fn (m1,m2) => fn ctxt => fn facts =>
+   let
+    val tac1 = method_evaluate m1 ctxt [] |> SELECT_GOAL 
+    val tac2 = method_evaluate m2 ctxt [] |> SELECT_GOAL
+   
+   in SIMPLE_METHOD' (tac1 THEN_ALL_NEW_FWD tac2) facts end)
+\<close>
+
+method repeat_all_new_fwd methods m = (then_all_new_fwd \<open>m\<close> \<open>(repeat_all_new_fwd \<open>m\<close>)?\<close>)
+
+
+method_setup focus_params_fixed =
+ \<open>Method.text_closure >> (fn m1src => fn ctxt => fn facts =>
+   let
+      val m1 = Method.evaluate_runtime m1src ctxt []
+      fun tac1 ctxt = NO_CONTEXT_TACTIC ctxt m1 
+   
+   in SIMPLE_METHOD' (Subgoal.FOCUS_PARAMS_FIXED (fn {context, ...} => tac1 context) ctxt) facts end)
+\<close>
+
+
+
+method_setup repeat =
+ \<open>Scan.lift Parse.nat -- Method.text_closure >> (fn (n,m) => fn ctxt => fn facts =>
+   let
+     fun tac st' = method_evaluate m ctxt facts st'
+
+   in SIMPLE_METHOD (REPEAT_DETERM_N n tac) facts end)
+\<close>
+
+method_setup repeat1 =
+ \<open>Scan.lift Parse.nat -- Method.text_closure >> (fn (n,m) => fn ctxt => fn facts =>
+   let
+     fun tac st' = method_evaluate m ctxt facts st'
+
+   in SIMPLE_METHOD (tac THEN REPEAT_DETERM_N (n-1) tac) facts end)
+\<close>
+
+method_setup parallel_all =
+ \<open>Method.text_closure >> (fn m => fn ctxt => fn facts =>
+   let
+     fun tac st' = method_evaluate m ctxt facts st'
+
+   in SIMPLE_METHOD (PARALLEL_GOALS tac) facts end)
+\<close>
+
+method_setup can =
+ \<open>Method.text_closure >> (fn m => fn ctxt => fn facts =>
+   let
+    fun CAN tac st =
+      case Seq.pull (tac st) of NONE => Seq.empty | _ => Seq.single st
+      
+     fun tac st' = method_evaluate m ctxt facts st'
+
+   in SIMPLE_METHOD (CAN tac) facts end)
+\<close>
+
+
+
+method_setup seqs = \<open>
+  let
+    fun SEQS abort_tac [] = all_tac
+      | SEQS abort_tac (m::ms) = m THEN_ELSE (SEQS abort_tac ms, abort_tac)
+  in
+    Method.text_closure --| Scan.lift @{keyword \<open>:\<close>} -- Scan.repeat1 Method.text_closure >> (fn (abm,ms) => fn ctxt => fn facts => let
+      val abort_tac = method_evaluate abm ctxt facts
+      val tacs = map (fn m => method_evaluate m ctxt facts) ms
+    in
+      SIMPLE_METHOD (SEQS abort_tac tacs) facts
+    end)
+  end
+\<close> \<open>\<open>seqs abort m\<^sub>1 ... m\<^sub>n\<close>: Execute as many of the given methods. If one fails, execute abort\<close>
+
+
+ML \<open>
+  structure More_Eisbach_Basic = struct
+    fun apply_method_noargs name ctxt =
+      NO_CONTEXT_TACTIC ctxt (Method_Closure.apply_method ctxt name [] [] [] ctxt [])
+      |> SELECT_GOAL;
+  end
+  
+  open More_Eisbach_Basic
+\<close>
+    
+end
